C code of Dijk23 were using old INF. So was dijkstra_constants. Changed. All versions of Prim need inf < MAX, because they use the PQ and the PQ needs inf+1 <= max. Added everywhere. Cleared the g2m Zlength PROP everywhere, including Prim. All of CAV is clean and admit-free

dijkstra/dijkstra_constants.v
@@ -1,13 +1,13 @@
 Require Import CertiGraph.dijkstra.dijkstra_env.
 
 Definition size := 8 : Z.
-Definition inf := 1879048193 : Z.
-(* Int.max_signed - Int.max_signed/size + 1 *)
+Definition inf := 2147483647 : Z.
+(* Int.max_signed *)
 
 Lemma size_eq: size = 8%Z.
 Proof. auto. Qed.
 
-Lemma inf_eq: inf = 1879048193%Z.
+Lemma inf_eq: inf = 2147483647%Z.
 Proof. auto. Qed.
 
 Global Opaque size.
